examples/ghc/module-edits/CoreFVs/preamble.v
@@ -1,3 +1,3 @@
-Require Import Core.
+
 
 
