examples/ghc/module-edits/Id/preamble.v
@@ -1,2 +1,2 @@
-Require Import Core.
+
 
