examples/ghc/module-edits/Var/preamble.v
@@ -1,1 +1,1 @@
-(* Require Import Core.*)
+
